FreydSSA/Ctx.lean
@@ -103,6 +103,11 @@ inductive Ctx.Wk {ν: Type u} {α: Type v} : Ctx ν α → Ctx ν α → Type (m
   | cons {Γ Δ} (x : Var ν α) : Ctx.Wk Γ Δ → Ctx.Wk (x::Γ) (x::Δ)
   | skip {Γ Δ} : Ctx.Fresh x.name Δ → Ctx.Wk Γ Δ → Ctx.Wk (x::Γ) Δ
 
+theorem Ctx.Wk.ty_eq {Γ : Ctx ν α} : Wk Γ [⟨x, A⟩] → Wk Γ [⟨x, A'⟩] → A = A'
+  | cons _ _, cons _ _ => rfl
+  | cons _ _, skip hx _ | skip hx _, cons _ _ => by cases hx; contradiction
+  | skip _ w, skip _ w' => w.ty_eq w'
+
 theorem Ctx.Wk.from_nil {ν α} {Γ : Ctx ν α} : Wk [] Γ → Γ = []
   | nil => rfl
 
